theories/examples/value_sensitivity_2.v
@@ -1,0 +1,124 @@
+(** Example from Ernst-Murray CAV 2019, done without locks. *)
+From iris.base_logic Require Import invariants.
+From iris_ni.logrel Require Import types.
+From iris_ni.program_logic Require Import dwp heap_lang_lifting.
+From iris.proofmode Require Import tactics.
+From iris.heap_lang Require Import lang proofmode.
+From iris_ni.proofmode Require Import dwp_tactics.
+From iris_ni.logrel Require Import interp value_dep.
+From iris_ni.examples Require Import lock par various (* for oneshot *).
+
+Definition thread1 : val :=
+  rec: "loop" "out" "rec" :=
+    (if: ~ is_classified "rec"
+     then "out" <- read_dep "rec"
+     else #());;
+    "loop" "out" "rec".
+
+Definition thread2 : val :=
+  λ: "rec", declassify "rec" #0.
+
+Definition prog : val := λ: "data" "out",
+  let: "rec" := (ref #true, ref "data") in
+  thread1 "out" "rec" ||| thread2 "rec".
+
+Section proof.
+  Context `{!heapDG Σ, !valueDepG Σ, !spawnG Σ, !oneshotG Σ}.
+
+  (* The invariant guarantees the monotonicity of the declassification. *)
+  Definition glinv γ γs :=
+    ((pending γs ∗ classification γ High (1/4))
+   ∨ (shot γs ∗ classification γ Low (1/4)))%I.
+
+  Definition N := nroot.@"blabla".
+
+  (* We verify that the thread that does the "dumping out" in a loop is secure,
+    under the monotonicity assumption. *)
+  Lemma thread1_spec γ γst γs out1 rec1 out2 rec2 ξ :
+    ⟦ tref (tint Low) ⟧ ξ out1 out2 -∗
+    value_dependent γ γst (tint Low) ξ rec1 rec2 -∗
+    inv N (glinv γ γs) -∗
+    DWP thread1 out1 rec1 & thread1 out2 rec2 : ⟦ tunit ⟧ ξ.
+  Proof.
+    iIntros "#Hout #Hvd #Hinv".
+    iLöb as "IH". dwp_rec. dwp_pures.
+    dwp_bind (is_classified _) (is_classified _).
+    iApply (is_classified_spec with "Hvd").
+    iIntros (α) "Ha".
+    iInv N as "[[Htok >Hc]|[#Htok >Hc]]" "Hcl";
+      iDestruct (classification_auth_agree with "[$Ha $Hc]") as %->;
+      iFrame "Ha".
+    + iMod ("Hcl" with "[Htok Hc]") as "_".
+      { iNext. iLeft. iFrame. }
+      iModIntro. iSimpl. dwp_pures. iApply "IH".
+    + iMod ("Hcl" with "[Htok Hc]") as "_".
+      { iNext. iRight. by iFrame. }
+      iModIntro. iSimpl. dwp_pures.
+      iApply (logrel_seq with "[-IH] IH").
+      dwp_bind (read_dep _) (read_dep _).
+      iApply (read_spec with "Hvd").
+      iIntros (α v1 v2) "Ha #Hv".
+      iInv N as "[[>Htok2 >Hc]|[_ >Hc]]" "Hcl".
+      { iExFalso. iApply (shot_not_pending with "Htok Htok2"). }
+      iDestruct (classification_auth_agree with "[$Ha $Hc]") as %->.
+      iFrame "Ha".
+      iMod ("Hcl" with "[Htok Hc]") as "_".
+      { iNext. iRight. by iFrame. }
+      iModIntro. iApply logrel_store; iApply dwp_value; eauto with iFrame.
+  Qed.
+
+  Lemma proof out1 out2 dat1 dat2 ξ :
+    ⟦ tref (tint Low) ⟧ ξ out1 out2 -∗
+    ⟦ tint High ⟧ ξ dat1 dat2 -∗
+    DWP (prog dat1 out1) & (prog dat2 out2) : ⟦ tprod tunit tunit ⟧ ξ.
+  Proof.
+    iIntros "#Hout #Hdat".
+    dwp_rec. dwp_pures.
+
+    dwp_bind (ref _)%E (ref _)%E.
+    iApply dwp_alloc. iIntros (rd1 rd2) "Hrd1 Hrd2". iNext.
+
+    dwp_bind (ref _)%E (ref _)%E.
+    iApply dwp_alloc. iIntros (is_classified1 is_classified2) "Hc1 Hc2". iNext.
+
+    iMod (make_value_dependent (tint Low) with "Hrd1 Hrd2 Hc1 Hc2 []")
+      as (γ γst) "[#Hvd Hc]".
+    { simpl. rewrite left_id. iExact "Hdat". }
+    iClear "Hdat".
+    dwp_pures.
+    iMod new_pending as (γs) "Hpend".
+
+    rewrite classification_quarter.
+    iDestruct "Hc" as "[Hc1 Hc]".
+
+    iMod (inv_alloc N _ (glinv γ γs) with "[-Hc]") as "#Hinv".
+    { iNext. iLeft. by iFrame. }
+
+    iApply (dwp_par (⟦ tunit ⟧ ξ) (⟦ tunit ⟧ ξ) with "[] [Hc]").
+    - (* Thread 1 *) iApply (thread1_spec with "Hout Hvd Hinv").
+    - (* Thread 2 *)
+      dwp_rec.
+      iApply (declassify_spec with "Hvd [] Hc").
+      { rewrite !interp_eq. iExists 0,0. by eauto. }
+      iIntros (α) "Ha Hf".
+      assert (Heq : ((3/4)%Qp + (1/4)%Qp)%Qp = 1%Qp).
+      { by apply (bool_decide_unpack _). }
+      iInv N as "[[>Htok >Hc]|[#Htok >Hc]]" "Hcl";
+        iDestruct (classification_auth_agree with "[$Ha $Hc]") as %->;
+        iCombine "Hf Hc" as "Hc"; rewrite Heq;
+        iMod (classification_update Low with "[$Ha $Hc]") as "[$ Hc]";
+        rewrite classification_quarter;
+        iDestruct "Hc" as "[Hc1 Hc]".
+      + iMod (shoot with "Htok") as "Htok".
+        iMod ("Hcl" with "[Htok Hc1]") as "_".
+        { iNext. iRight. by iFrame. }
+        iModIntro. eauto.
+      + iMod ("Hcl" with "[Htok Hc1]") as "_".
+        { iNext. iRight. by iFrame. }
+        iModIntro. eauto.
+    - (* Finally *)
+      iIntros (???? [-> ->] [-> ->]).
+      iNext. iExists _,_,_,_; eauto with iFrame.
+  Qed.
+
+End proof.
